ind/DoublyLinkedListIface.fsti
@@ -258,3 +258,11 @@ val dll_remove_mid (d:dll 'a) (n:node 'a) :
 // + If node is in valid list, it is also valid
 // + If node is in list, fp is included
 // + If node is not in list, fp is disjoint
+
+val _auto_node_in_valid_dll_is_valid (h:HS.mem) (d:dll 'a) (n:node 'a) :
+  Lemma
+    (requires (dll_valid h d /\ n `L.memP` as_list h d))
+    (ensures (node_valid h n))
+    [SMTPat (dll_valid h d);
+     SMTPat (n `L.memP` as_list h d);
+     SMTPat (node_valid h n)]
